src/named/SimpleVCPS.v
@@ -16,54 +16,8 @@ Require Coq.derive.Derive.
 Local Notation compiler := (compiler string).
 
 
-Definition block_subst_def : lang :=
-  {[l
-      [s| "G" : #"env"
-          -----------------------------------------------
-          #"blk" "G" srt
-      ];
-  [:| "G" : #"env", "G'" : #"env", "g" : #"sub" "G" "G'",
-      "e" : #"blk" "G'"
-       -----------------------------------------------
-       #"blk_subst" "g" "e" : #"blk" "G"
-  ];
-  [:= "G" : #"env", "e" : #"blk" "G"
-       ----------------------------------------------- ("blk_subst_id")
-       #"blk_subst" #"id" "e" = "e" : #"blk" "G"
-  ]; 
-  [:= "G1" : #"env", "G2" : #"env", "G3" : #"env",
-       "f" : #"sub" "G1" "G2", "g" : #"sub" "G2" "G3",
-       "e" : #"blk" "G3"
-       ----------------------------------------------- ("blk_subst_cmp")
-       #"blk_subst" "f" (#"blk_subst" "g" "e")
-       = #"blk_subst" (#"cmp" "f" "g") "e"
-       : #"blk" "G1"
-  ]
-  (*TODO: any reason to add halt?
-  [:| "G" : #"env", "v" : #"val" "G" "A"
-       -----------------------------------------------
-       #"ret" "v" : #"blk" "G" "A"
-  ];
-   
-  [:= "G1" : #"env", "G2" : #"env",
-       "g" : #"sub" "G1" "G2",
-       "A" : #"ty", "v" : #"val" "G2" "A"
-       ----------------------------------------------- ("blk_subst_ret")
-       #"blk_subst" "g" (#"ret" "v")
-       = #"ret" (#"val_subst" "g" "v")
-       : #"blk" "G1" "A"
-  ]*)
-  ]}.
-
-Derive block_subst
-       SuchThat (elab_lang_ext value_subst block_subst_def block_subst)
-       As block_subst_wf.
-Proof. auto_elab. Qed.
-#[export] Hint Resolve block_subst_wf : elab_pfs.
-
-
 Definition cps_lang_def : lang :=
-  {[l
+  {[l/subst
       [:| "A" : #"ty"
           -----------------------------------------------
           #"neg" "A" : #"ty"
@@ -97,29 +51,8 @@ Definition cps_lang_def : lang :=
       #"cont" "A" (#"jmp" (#"val_subst" #"wkn" "v") #"hd")
       = "v"
       : #"val" "G" (#"neg" "A")
-  ];
-  [:= "G" : #"env", "A" : #"ty",
-      "v1" : #"val" "G" (#"neg" "A"),
-      "v2" : #"val" "G" "A",
-      "G'" : #"env",
-      "g" : #"sub" "G'" "G"
-      ----------------------------------------------- ("jmp_subst")
-      #"blk_subst" "g" (#"jmp" "v1" "v2")
-      = #"jmp" (#"val_subst" "g" "v1") (#"val_subst" "g" "v2")
-      : #"blk" "G'"
-  ];  
-  [:= "G" : #"env", "A" : #"ty",
-      "e" : #"blk" (#"ext" "G" "A"),
-      "G'" : #"env",
-      "g" : #"sub" "G'" "G"
-      ----------------------------------------------- ("cont_subst")
-      #"val_subst" "g" (#"cont" "A" "e")
-      = #"cont" "A" (#"blk_subst"
-                       (#"snoc" (#"cmp" #"wkn" "g") #"hd") "e")
-      : #"val" "G'" (#"neg" "A")
   ]
   ]}.
-
 
 Derive cps_lang
        SuchThat (elab_lang_ext (block_subst ++ value_subst)
@@ -179,7 +112,7 @@ Proof. auto_elab_compiler. Qed.
 
 (*TODO: separate file?*)
 Definition cps_prod_lang_def : lang :=
-  {[l
+  {[l/subst
       
   [:| "A" : #"ty", "B": #"ty"
       -----------------------------------------------
@@ -219,29 +152,7 @@ Definition cps_prod_lang_def : lang :=
       #"pm_pair" "v" (#"blk_subst" (#"snoc" (#"cmp" #"wkn" #"wkn") (#"pair" {ovar 1} {ovar 0})) "e")
       = #"blk_subst" (#"snoc" #"id" "v") "e"
       : #"blk" "G"
-  ];
-  [:= "G" : #"env", "A" : #"ty", "B" : #"ty",
-      "e" : #"val" "G" "A",
-      "e'" : #"val" "G" "B",
-      "G'" : #"env",
-      "g" : #"sub" "G'" "G"
-      ----------------------------------------------- ("pair_subst")
-      #"val_subst" "g" (#"pair" "e" "e'")
-      = #"pair" (#"val_subst" "g" "e") (#"val_subst" "g" "e'")
-      : #"val" "G'" (#"prod" "A" "B")
-  ];
-  [:= "G" : #"env", "A" : #"ty", "B" : #"ty",
-      "v" : #"val" "G" (#"prod" "A" "B"),
-      "e" : #"blk" (#"ext" (#"ext" "G" "A") "B"),
-      "G'" : #"env",
-      "g" : #"sub" "G'" "G"
-      ----------------------------------------------- ("pm_pair_subst")
-      #"blk_subst" "g" (#"pm_pair" "v" "e")
-      = #"pm_pair" (#"val_subst" "g" "v")
-         (#"blk_subst" (#"snoc" (#"cmp" #"wkn" (#"snoc" (#"cmp" #"wkn" "g") #"hd")) #"hd") "e")
-      : #"blk" "G'"
-  ]
-  ]}.
+  ] ]}.
 
 
     
